---
title: 'Exercise 10.1.1a'
author: 'Nathan Lunceford'
format:
  html:
    self-contained: true
    page-layout: full
    toc: true
    toc-depth: 1
    toc-location: right
    number-sections: false
    html-math-method: katex
    embed-resources: true
    code-fold: true
    code-summary: 'Show the code'
    code-overflow: wrap
    code-copy: hover
    code-tools:
      source: false
      toggle: true
      caption: See code
engine: jupyter
preview:
  port: 3000
  browser: true
  watch-inputs: true
  navigate: true
---

# **Problem**

::: {.callout-note icon=false }

## **10.1.1a**

Find the Discrete Fourier Transform (DFT) of the following vector:

$$
\begin{bmatrix}
0 \\ 1 \\ 0 \\ -1
\end{bmatrix}
$$

:::

# **Solution**

## **DFT of $[0, 1, 0, -1]^T$**

### Define Parameters

The vector has $n = 4$, so:

$$
\omega = e^{-i \frac{2\pi}{4}} = i
$$

The formula for the DFT is:

$$
y_k = \frac{1}{\sqrt{n}} \sum_{j=0}^{n-1} x_j \omega^{jk}, \quad k = 0, 1, \dots, n-1
$$

### Compute Each $y_k$:

1. **$y_0$:**

   $$
   y_0 = \frac{1}{\sqrt{4}} \sum_{j=0}^{3} x_j \omega^{j \cdot 0} = \frac{1}{2}(0 + 1 + 0 - 1) = 0
   $$

2. **$y_1$:**

   $$
   y_1 = \frac{1}{\sqrt{4}} \sum_{j=0}^{3} x_j \omega^{j \cdot 1} = \frac{1}{2}(0 + i \cdot 1 + 0 + (-1) \cdot (-i)) = \frac{1}{2}(i + i) = i
   $$

3. **$y_2$:**

   $$
   y_2 = \frac{1}{\sqrt{4}} \sum_{j=0}^{3} x_j \omega^{j \cdot 2} = \frac{1}{2}(0 + (-1) + 0 + (-1)) = -1
   $$

4. **$y_3$:**
   $$
   y_3 = \frac{1}{\sqrt{4}} \sum_{j=0}^{3} x_j \omega^{j \cdot 3} = \frac{1}{2}(0 + (-i) + 0 + (-1) \cdot i) = \frac{1}{2}(-i - i) = -i
   $$

### Result:

The DFT of $[0, 1, 0, -1]$ is:

$$
y = [0, i, -1, -i]
$$
